src/case_study/program_logic/cl_weakestpre.v
@@ -14,9 +14,9 @@ Section clwp_def.
   Context {expr val ectx state observation} {Λ : CCEctxLanguage expr val ectx state observation}.
   Context `{irisGS_gen hlc (CC_ectx_lang expr) Σ}.
 
-Definition clwp_def (E : coPset) (e : expr) (a : A) (Φ : val → iProp Σ) : iProp Σ :=
-  (∀ K Ψ, (∀ v, Φ v -∗ WP fill K (of_val v) @ (NotStuck,a); E {{Ψ}})
-            -∗ WP fill K e @ (NotStuck,a); E {{Ψ}})%I.
+Definition clwp_def (E : coPset) (e : expr) (Φ : val → iProp Σ) : iProp Σ :=
+  (∀ K Ψ, (∀ v, Φ v -∗ WP fill K (of_val v) @ E {{Ψ}})
+            -∗ WP fill K e @ E {{Ψ}})%I.
 Definition clwp_aux : seal (@clwp_def). by eexists. Qed.
 Definition clwp := unseal clwp_aux.
 Definition clwp_eq : @clwp = @clwp_def := seal_eq clwp_aux.
@@ -26,19 +26,19 @@ End clwp_def.
 Instance: Params (@clwp) 7.
 Defined.
 
-Notation "'CLWP' e @ a ; E {{ Φ } }" := (clwp E e%E a Φ)
+Notation "'CLWP' e @ E {{ Φ } }" := (clwp E e%E Φ)
   (at level 20, e, Φ at level 200,
-   format "'CLWP'  e  @  a  ;  E  {{  Φ  } }") : bi_scope.
-Notation "'CLWP' e @ a {{ Φ } }" := (clwp ⊤ e%E a Φ)
+   format "'CLWP'  e  @  E  {{  Φ  } }") : bi_scope.
+Notation "'CLWP' e {{ Φ } }" := (clwp ⊤ e%E Φ)
   (at level 20, e, Φ at level 200,
-   format "'CLWP'  e  @  a  {{  Φ  } }") : bi_scope.
+   format "'CLWP'  e  {{  Φ  } }") : bi_scope.
 
-Notation "'CLWP' e @ a ; E {{ v , Q } }" := (clwp E e%E a (λ v, Q))
+Notation "'CLWP' e @ E {{ v , Q } }" := (clwp E e%E (λ v, Q))
   (at level 20, e, Q at level 200,
-   format "'CLWP'  e  @  a  ;  E  {{  v ,  Q  } }") : bi_scope.
-Notation "'CLWP' e @ a {{ v , Q } }" := (clwp ⊤ e%E a (λ v, Q))
+   format "'CLWP'  e  @  E  {{  v ,  Q  } }") : bi_scope.
+Notation "'CLWP' e {{ v , Q } }" := (clwp ⊤ e%E (λ v, Q))
   (at level 20, e, Q at level 200,
-   format "'CLWP'  e  @  a  {{  v ,  Q  } }") : bi_scope.
+   format "'CLWP'  e  {{  v ,  Q  } }") : bi_scope.
 
 Section clwp.
   Context {expr val ectx state observation} {Λ : CCEctxLanguage expr val ectx state observation}.
@@ -48,23 +48,22 @@ Section clwp.
   Implicit Types Φ Ψ : val → iProp Σ.
   Implicit Types v : val.
   Implicit Types e : expr.
-  Implicit Types a : A.
   
-  Lemma clwp_cl {E e a Φ} K :
-    CLWP e @ a; E {{Φ}} -∗
-    (∀ Ψ, (∀ v, Φ v -∗ WP fill K (of_val v) @ (NotStuck,a); E {{Ψ}})
-            -∗ WP fill K e @ (NotStuck,a); E {{Ψ}})%I.
+  Lemma clwp_cl {E e Φ} K :
+    CLWP e @ E {{Φ}} -∗
+    (∀ Ψ, (∀ v, Φ v -∗ WP fill K (of_val v) @ E {{Ψ}})
+            -∗ WP fill K e @ E {{Ψ}})%I.
   Proof. rewrite clwp_eq /clwp_def. iIntros "H". iIntros (?). iApply "H". Qed.
 
   (* Weakest pre *)
-  Lemma unfold_clwp (E : coPset) (e : expr) (a : A) (Φ : val → iProp Σ) :
-    CLWP e @ a; E {{Φ}} ⊣⊢
-         (∀ K Ψ, (∀ v, Φ v -∗ WP fill K (of_val v) @ (NotStuck,a); E {{Ψ}})
-                   -∗ WP fill K e @ (NotStuck,a); E {{Ψ}})%I.
+  Lemma unfold_clwp (E : coPset) (e : expr) (Φ : val → iProp Σ) :
+    CLWP e @ E {{Φ}} ⊣⊢
+         (∀ K Ψ, (∀ v, Φ v -∗ WP fill K (of_val v) @ E {{Ψ}})
+                   -∗ WP fill K e @ E {{Ψ}})%I.
   Proof. by rewrite clwp_eq /clwp_def. Qed.
 
-  Lemma clwp_wp (E : coPset) (e : expr) (a : A) (Φ : val → iProp Σ) :
-    CLWP e @ a; E {{Φ}} ⊢ WP e @ (NotStuck,a); E {{Φ}}.
+  Lemma clwp_wp (E : coPset) (e : expr) (Φ : val → iProp Σ) :
+    CLWP e @ E {{Φ}} ⊢ WP e @ E {{Φ}}.
   Proof.
     iIntros "H". rewrite unfold_clwp.
     iSpecialize ("H" $! empty_ectx Φ with "[]").
@@ -73,41 +72,41 @@ Section clwp.
     - by rewrite CC_fill_empty.
   Qed.
 
-  Global Instance clwp_ne E e a n :
-    Proper (pointwise_relation _ (dist n) ==> dist n) (@clwp _ _ _ _ _ Λ _ Σ _ E e a).
+  Global Instance clwp_ne E e n :
+    Proper (pointwise_relation _ (dist n) ==> dist n) (@clwp _ _ _ _ _ Λ _ Σ _ E e).
   Proof.
     repeat intros?; rewrite !unfold_clwp.
     repeat (repeat apply forall_ne=>?; repeat apply wand_ne; trivial).
   Qed.
-  Global Instance clwp_proper E e a :
-    Proper (pointwise_relation _ (≡) ==> (≡)) (@clwp _ _ _ _ _ Λ _ Σ _ E e a).
+  Global Instance clwp_proper E e :
+    Proper (pointwise_relation _ (≡) ==> (≡)) (@clwp _ _ _ _ _ Λ _ Σ _ E e).
   Proof.
       by intros Φ Φ' ?; apply equiv_dist=>n; apply clwp_ne=>v; apply equiv_dist.
   Qed.
 
-  Lemma clwp_value' E Φ v a : Φ v ⊢ CLWP of_val v @ a; E {{ Φ }}.
+  Lemma clwp_value' E Φ v : Φ v ⊢ CLWP of_val v @ E {{ Φ }}.
   Proof.
     iIntros "HΦ"; rewrite unfold_clwp.
     iIntros (K Ψ) "HK". iApply ("HK" with "HΦ").
   Qed.
-  Lemma clwp_value_inv E Φ v a : CLWP of_val v @ a; E {{ Φ }} ={E}=∗ Φ v.
+  Lemma clwp_value_inv E Φ v : CLWP of_val v @ E {{ Φ }} ={E}=∗ Φ v.
   Proof. iIntros "H"; iApply wp_value_fupd'. by iApply clwp_wp. Qed.
 
-  Lemma fupd_clwp E e Φ a : (|={E}=> CLWP e @ a; E {{ Φ }}) ⊢ CLWP e @ a; E {{ Φ }}.
+  Lemma fupd_clwp E e Φ : (|={E}=> CLWP e @ E {{ Φ }}) ⊢ CLWP e @ E {{ Φ }}.
   Proof.
     iIntros "H"; rewrite !unfold_clwp.
     iIntros (K Ψ) "HK". iMod "H"; by iApply "H".
   Qed.
-  Lemma clwp_fupd E e Φ a : CLWP e @ a; E {{ v, |={E}=> Φ v }} ⊢ CLWP e @ a; E {{ Φ }}.
+  Lemma clwp_fupd E e Φ : CLWP e @ E {{ v, |={E}=> Φ v }} ⊢ CLWP e @ E {{ Φ }}.
   Proof.
     iIntros "H"; rewrite !unfold_clwp.
     iIntros (K Ψ) "HK".
     iApply "H". iIntros (w) ">Hw"; by iApply "HK".
   Qed.
 
-  Lemma clwp_bind K E e Φ a :
-    CLWP e @ a; E {{ v, CLWP fill K (of_val v) @ a; E {{ Φ }} }}
-    ⊢ CLWP fill K e @ a; E {{ Φ }}.
+  Lemma clwp_bind K E e Φ :
+    CLWP e @ E {{ v, CLWP fill K (of_val v) @ E {{ Φ }} }}
+    ⊢ CLWP fill K e @ E {{ Φ }}.
   Proof.
     iIntros "H"; rewrite !unfold_clwp. iIntros (K' Ψ) "HK'".
     rewrite CC_fill_comp.
@@ -118,50 +117,50 @@ Section clwp.
   Qed.
 
   (** * Derived rules *)
-  Lemma clwp_mono E e a Φ Ψ : (∀ v, Φ v ⊢ Ψ v) →
-    CLWP e @ a; E {{ Φ }} ⊢ CLWP e @ a; E {{ Ψ }}.
+  Lemma clwp_mono E e Φ Ψ : (∀ v, Φ v ⊢ Ψ v) →
+    CLWP e @ E {{ Φ }} ⊢ CLWP e @ E {{ Ψ }}.
   Proof.
     iIntros (HΦ) "H"; rewrite !unfold_clwp. iIntros (K χ) "HK".
     iApply "H". iIntros (w) "Hw". iApply "HK"; by iApply HΦ.
   Qed.
-  Global Instance clwp_mono' E e a :
-    Proper (pointwise_relation _ (⊢) ==> (⊢)) (@clwp _ _ _ _ _ Λ _ Σ _ E e a).
+  Global Instance clwp_mono' E e :
+    Proper (pointwise_relation _ (⊢) ==> (⊢)) (@clwp _ _ _ _ _ Λ _ Σ _ E e).
   Proof. by intros Φ Φ' ?; apply clwp_mono. Qed.
 
-  Lemma clwp_value E Φ e a v `{!IntoVal e v} : Φ v ⊢ CLWP e @ a; E {{ Φ }}.
+  Lemma clwp_value E Φ e v `{!IntoVal e v} : Φ v ⊢ CLWP e @ E {{ Φ }}.
   Proof. intros; rewrite -(of_to_val e v) //. by apply clwp_value'. rewrite /IntoVal /= in IntoVal0.
          rewrite -to_of_val IntoVal0 //. Qed.
-  Lemma clwp_value_fupd' E Φ a v : (|={E}=> Φ v) ⊢ CLWP of_val v @ a; E {{ Φ }}.
+  Lemma clwp_value_fupd' E Φ v : (|={E}=> Φ v) ⊢ CLWP of_val v @ E {{ Φ }}.
   Proof. intros. by rewrite -clwp_fupd -clwp_value'. Qed.
-  Lemma clwp_value_fupd E Φ e v a `{!IntoVal e v} :
-    (|={E}=> Φ v) ⊢ CLWP e @ a; E {{ Φ }}.
+  Lemma clwp_value_fupd E Φ e v `{!IntoVal e v} :
+    (|={E}=> Φ v) ⊢ CLWP e @ E {{ Φ }}.
   Proof. intros. rewrite -clwp_fupd -clwp_value //. Qed.
 
-  Lemma clwp_frame_l E a e Φ R :
-    R ∗ CLWP e @ a; E {{ Φ }} ⊢ CLWP e @ a; E {{ v, R ∗ Φ v }}.
+  Lemma clwp_frame_l E e Φ R :
+    R ∗ CLWP e @ E {{ Φ }} ⊢ CLWP e @ E {{ v, R ∗ Φ v }}.
   Proof.
     iIntros "[HR H]"; rewrite !unfold_clwp. iIntros (K Ψ) "HK".
     iApply "H". iIntros (v) "Hv". iApply "HK"; iFrame.
   Qed.
-  Lemma clwp_frame_r E a e Φ R :
-    CLWP e @ a; E {{ Φ }} ∗ R ⊢ CLWP e @ a; E {{ v, Φ v ∗ R }}.
+  Lemma clwp_frame_r E e Φ R :
+    CLWP e @ E {{ Φ }} ∗ R ⊢ CLWP e @ E {{ v, Φ v ∗ R }}.
   Proof.
     iIntros "[H HR]"; rewrite !unfold_clwp. iIntros (K Ψ) "HK".
     iApply "H". iIntros (v) "Hv". iApply "HK"; iFrame.
   Qed.
 
-  Lemma clwp_wand E e a Φ Ψ :
-    CLWP e @ a; E {{ Φ }} -∗ (∀ v, Φ v -∗ Ψ v) -∗ CLWP e @ a; E {{ Ψ }}.
+  Lemma clwp_wand E e Φ Ψ :
+    CLWP e @ E {{ Φ }} -∗ (∀ v, Φ v -∗ Ψ v) -∗ CLWP e @ E {{ Ψ }}.
   Proof.
     iIntros "Hwp H". rewrite !unfold_clwp.
     iIntros (K χ) "HK".
     iApply "Hwp". iIntros (?) "?"; iApply "HK"; by iApply "H".
   Qed.
-  Lemma clwp_wand_l E e a Φ Ψ :
-    (∀ v, Φ v -∗ Ψ v) ∗ CLWP e @ a; E {{ Φ }} ⊢ CLWP e @ a; E {{ Ψ }}.
+  Lemma clwp_wand_l E e Φ Ψ :
+    (∀ v, Φ v -∗ Ψ v) ∗ CLWP e @ E {{ Φ }} ⊢ CLWP e @ E {{ Ψ }}.
   Proof. iIntros "[H Hwp]". iApply (clwp_wand with "Hwp H"). Qed.
-  Lemma clwp_wand_r E e a Φ Ψ :
-    CLWP e @ a; E {{ Φ }} ∗ (∀ v, Φ v -∗ Ψ v) ⊢ CLWP e @ a; E {{ Ψ }}.
+  Lemma clwp_wand_r E e Φ Ψ :
+    CLWP e @ E {{ Φ }} ∗ (∀ v, Φ v -∗ Ψ v) ⊢ CLWP e @ E {{ Ψ }}.
   Proof. iIntros "[Hwp H]". iApply (clwp_wand with "Hwp H"). Qed.
 End clwp.
 
@@ -172,23 +171,23 @@ Section proofmode_classes.
   Implicit Types P Q : iProp Σ.
   Implicit Types Φ : val → iProp Σ.
 
-  Global Instance frame_clwp p E e R Φ Ψ a :
+  Global Instance frame_clwp p E e R Φ Ψ :
     (∀ v, Frame p R (Φ v) (Ψ v)) →
-    Frame p R (CLWP e @ a; E {{ Φ }}) (CLWP e @ a; E {{ Ψ }}).
+    Frame p R (CLWP e @ E {{ Φ }}) (CLWP e @ E {{ Ψ }}).
   Proof. rewrite /Frame=> HR. rewrite clwp_frame_l. apply clwp_mono, HR. Qed.
 
-  Global Instance is_except_0_clwp E e a Φ : IsExcept0 (CLWP e @ a; E {{ Φ }}).
+  Global Instance is_except_0_clwp E e Φ : IsExcept0 (CLWP e @ E {{ Φ }}).
   Proof. by rewrite /IsExcept0 -{2}fupd_clwp -except_0_fupd -fupd_intro. Qed.
 
-  Global Instance elim_modal_bupd_clwp p E e a P Φ :
-    ElimModal True p false (|==> P) P (CLWP e @ a; E {{ Φ }}) (CLWP e @ a; E {{ Φ }}).
+  Global Instance elim_modal_bupd_clwp p E e P Φ :
+    ElimModal True p false (|==> P) P (CLWP e @ E {{ Φ }}) (CLWP e @ E {{ Φ }}).
   Proof.
       by rewrite /ElimModal intuitionistically_if_elim
                  (bupd_fupd E) fupd_frame_r wand_elim_r fupd_clwp.
   Qed.
 
-  Global Instance elim_modal_fupd_clwp p E e a P Φ :
-    ElimModal True p false (|={E}=> P) P (CLWP e @ a; E {{ Φ }}) (CLWP e @ a; E {{ Φ }}).
+  Global Instance elim_modal_fupd_clwp p E e P Φ :
+    ElimModal True p false (|={E}=> P) P (CLWP e @ E {{ Φ }}) (CLWP e @ E {{ Φ }}).
   Proof.
       by rewrite /ElimModal intuitionistically_if_elim
                  fupd_frame_r wand_elim_r fupd_clwp.
