src/case_study/program_logic/lifting.v
@@ -7,7 +7,7 @@ From iris.prelude Require Import options.
 
 Section lifting.
 Context `{!irisGS_gen hlc Λ Σ}.
-Implicit Types s : (stuckness * A).
+Implicit Types s : (stuckness).
 Implicit Types v : val Λ.
 Implicit Types e : expr Λ.
 Implicit Types σ : state Λ.
@@ -19,12 +19,12 @@ Local Hint Resolve reducible_no_obs_reducible : core.
 Lemma wp_lift_step_fupdN s E Φ e1 :
   to_val e1 = None →
   (∀ σ1 ns κ κs nt, (state_interp σ1 ns (κ ++ κs) nt) ={E,∅}=∗
-    ⌜if s.1 is NotStuck then reducible e1 σ1 else True⌝ ∗
+    ⌜if s is NotStuck then reducible e1 σ1 else True⌝ ∗
     ∀ e2 σ2 efs, ⌜prim_step e1 σ1 κ e2 σ2 efs⌝ -∗
       £ (S $ num_laters_per_step ns)
       ={∅}▷=∗^(S $ num_laters_per_step ns) |={∅,E}=>
       state_interp σ2 (S ns) κs (length efs + nt) ∗
-      (⚡={next_state (next_a e1 s.2)}=> WP e2 @ s; E {{ Φ }}) ∗
+      (⚡={next_state e1}=> WP e2 @ s; E {{ Φ }}) ∗
       [∗ list] ef ∈ efs, WP ef @ s; ⊤ {{ fork_post }})
   ⊢ WP e1 @ s; E {{ Φ }}.
 Proof. by rewrite wp_unfold /wp_pre=>->. Qed.
@@ -32,10 +32,10 @@ Proof. by rewrite wp_unfold /wp_pre=>->. Qed.
 Lemma wp_lift_step_fupd s E Φ e1 :
   to_val e1 = None →
   (∀ σ1 ns κ κs nt, (state_interp σ1 ns (κ ++ κs) nt) ={E,∅}=∗
-    ⌜if s.1 is NotStuck then reducible e1 σ1 else True⌝ ∗
+    ⌜if s is NotStuck then reducible e1 σ1 else True⌝ ∗
     ∀ e2 σ2 efs, ⌜prim_step e1 σ1 κ e2 σ2 efs⌝ -∗ £ 1 ={∅}=∗ ▷ |={∅,E}=>
       (state_interp σ2 (S ns) κs (length efs + nt)) ∗
-      (⚡={next_state (next_a e1 s.2)}=> WP e2 @ s; E {{ Φ }}) ∗
+      (⚡={next_state e1}=> WP e2 @ s; E {{ Φ }}) ∗
       [∗ list] ef ∈ efs, WP ef @ s; ⊤ {{ fork_post }})
   ⊢ WP e1 @ s; E {{ Φ }}.
 Proof.
@@ -48,24 +48,24 @@ Proof.
   iApply step_fupd_intro; done.
 Qed.
 
-(* Lemma wp_lift_stuck E Φ e : *)
-(*   to_val e = None → *)
-(*   (∀ σ ns κs nt, (state_interp σ ns κs nt) ={E,∅}=∗ ⌜stuck e σ⌝) *)
-(*   ⊢ WP e @ E ?{{ Φ }}. *)
-(* Proof. *)
-(*   rewrite wp_unfold /wp_pre=>->. iIntros "H" (σ1 ns κ κs nt) "Hσ". *)
-(*   iMod ("H" with "Hσ") as %[? Hirr]. iModIntro. iSplit; first done. *)
-(*   iIntros (e2 σ2 efs ?). by case: (Hirr κ e2 σ2 efs). *)
-(* Qed. *)
+Lemma wp_lift_stuck E Φ e :
+  to_val e = None →
+  (∀ σ ns κs nt, (state_interp σ ns κs nt) ={E,∅}=∗ ⌜stuck e σ⌝)
+  ⊢ WP e @ E ?{{ Φ }}.
+Proof.
+  rewrite wp_unfold /wp_pre=>->. iIntros "H" (σ1 ns κ κs nt) "Hσ".
+  iMod ("H" with "Hσ") as %[? Hirr]. iModIntro. iSplit; first done.
+  iIntros (e2 σ2 efs ?). by case: (Hirr κ e2 σ2 efs).
+Qed.
 
 (** Derived lifting lemmas. *)
 Lemma wp_lift_step s E Φ e1 :
   to_val e1 = None →
   (∀ σ1 ns κ κs nt, (state_interp σ1 ns (κ ++ κs) nt) ={E,∅}=∗
-    ⌜if s.1 is NotStuck then reducible e1 σ1 else True⌝ ∗
+    ⌜if s is NotStuck then reducible e1 σ1 else True⌝ ∗
     ▷ ∀ e2 σ2 efs, ⌜prim_step e1 σ1 κ e2 σ2 efs⌝ -∗ £ 1 ={∅,E}=∗
       (state_interp σ2 (S ns) κs (length efs + nt)) ∗
-      (⚡={next_state (next_a e1 s.2)}=> WP e2 @ s; E {{ Φ }}) ∗
+      (⚡={next_state e1}=> WP e2 @ s; E {{ Φ }}) ∗
       [∗ list] ef ∈ efs, WP ef @ s; ⊤ {{ fork_post }})
   ⊢ WP e1 @ s; E {{ Φ }}.
 Proof.
@@ -74,16 +74,16 @@ Proof.
 Qed.
 
 Lemma wp_lift_pure_step_no_fork `{!Inhabited (state Λ)} s E E' Φ e1 :
-  (∀ σ1, if s.1 is NotStuck then reducible e1 σ1 else to_val e1 = None) →
+  (∀ σ1, if s is NotStuck then reducible e1 σ1 else to_val e1 = None) →
   (∀ κ σ1 e2 σ2 efs, prim_step e1 σ1 κ e2 σ2 efs → κ = [] ∧ σ2 = σ1 ∧ efs = []) →
-  (|={E}[E']▷=> ∀ κ e2 efs σ, ⌜prim_step e1 σ κ e2 σ efs⌝ -∗ £ 1 -∗ ⚡={next_state (next_a e1 s.2)}=> WP e2 @ s; E {{ Φ }})
+  (|={E}[E']▷=> ∀ κ e2 efs σ, ⌜prim_step e1 σ κ e2 σ efs⌝ -∗ £ 1 -∗ ⚡={next_state e1}=> WP e2 @ s; E {{ Φ }})
   ⊢ WP e1 @ s; E {{ Φ }}.
 Proof.
   iIntros (Hsafe Hstep) "H". iApply wp_lift_step.
-  { specialize (Hsafe inhabitant). destruct s as [s a];simpl in *;destruct s; eauto using reducible_not_val. }
+  { specialize (Hsafe inhabitant). destruct s; eauto using reducible_not_val. }
   iIntros (σ1 ns κ κs nt) "Hσ". iMod "H".
   iApply fupd_mask_intro; first set_solver. iIntros "Hclose". iSplit.
-  { iPureIntro. destruct s as [s a];simpl in *;destruct s; done. }
+  { iPureIntro. destruct s; done. }
   iNext. iIntros (e2 σ2 efs ?) "Hcred".
   destruct (Hstep κ σ1 e2 σ2 efs) as (-> & <- & ->); auto.
   iMod "Hclose" as "_". iMod "H". iModIntro.
@@ -92,25 +92,25 @@ Proof.
   by iApply state_interp_mono.
 Qed.
 
-(* Lemma wp_lift_pure_stuck `{!Inhabited (state Λ)} E Φ e : *)
-(*   (∀ σ, stuck e σ) → *)
-(*   True ⊢ WP e @ E ?{{ Φ }}. *)
-(* Proof. *)
-(*   iIntros (Hstuck) "_". iApply wp_lift_stuck. *)
-(*   - destruct(to_val e) as [v|] eqn:He; last done. *)
-(*     rewrite -He. by case: (Hstuck inhabitant). *)
-(*   - iIntros (σ ns κs nt) "_". iApply fupd_mask_intro; auto with set_solver. *)
-(* Qed. *)
+Lemma wp_lift_pure_stuck `{!Inhabited (state Λ)} E Φ e :
+  (∀ σ, stuck e σ) →
+  True ⊢ WP e @ E ?{{ Φ }}.
+Proof.
+  iIntros (Hstuck) "_". iApply wp_lift_stuck.
+  - destruct(to_val e) as [v|] eqn:He; last done.
+    rewrite -He. by case: (Hstuck inhabitant).
+  - iIntros (σ ns κs nt) "_". iApply fupd_mask_intro; auto with set_solver.
+Qed.
 
 (* Atomic steps don't need any mask-changing business here, one can
    use the generic lemmas here. *)
 Lemma wp_lift_atomic_step_fupd {s E1 E2 Φ} e1 :
   to_val e1 = None →
   (∀ σ1 ns κ κs nt, (state_interp σ1 ns (κ ++ κs) nt) ={E1}=∗
-    ⌜if s.1 is NotStuck then reducible e1 σ1 else True⌝ ∗
+    ⌜if s is NotStuck then reducible e1 σ1 else True⌝ ∗
     ∀ e2 σ2 efs, ⌜prim_step e1 σ1 κ e2 σ2 efs⌝ -∗ £ 1 ={E1}[E2]▷=∗
       (state_interp σ2 (S ns) κs (length efs + nt)) ∗
-      from_option (λ v, ⚡={next_state (next_a e1 s.2)}=> Φ v) False (to_val e2) ∗
+      from_option (λ v, ⚡={next_state e1}=> Φ v) False (to_val e2) ∗
       [∗ list] ef ∈ efs, WP ef @ s; ⊤ {{ fork_post }})
   ⊢ WP e1 @ s; E1 {{ Φ }}.
 Proof.
@@ -129,10 +129,10 @@ Qed.
 Lemma wp_lift_atomic_step {s E Φ} e1 :
   to_val e1 = None →
   (∀ σ1 ns κ κs nt, (state_interp σ1 ns (κ ++ κs) nt) ={E}=∗
-    ⌜if s.1 is NotStuck then reducible e1 σ1 else True⌝ ∗
+    ⌜if s is NotStuck then reducible e1 σ1 else True⌝ ∗
     ▷ ∀ e2 σ2 efs, ⌜prim_step e1 σ1 κ e2 σ2 efs⌝ -∗ £ 1 ={E}=∗
       (state_interp σ2 (S ns) κs (length efs + nt)) ∗
-      from_option (λ v, ⚡={next_state (next_a e1 s.2)}=> Φ v) False (to_val e2) ∗
+      from_option (λ v, ⚡={next_state e1}=> Φ v) False (to_val e2) ∗
       [∗ list] ef ∈ efs, WP ef @ s; ⊤ {{ fork_post }})
   ⊢ WP e1 @ s; E {{ Φ }}.
 Proof.
@@ -143,10 +143,10 @@ Proof.
 Qed.
 
 Lemma wp_lift_pure_det_step_no_fork `{!Inhabited (state Λ)} {s E E' Φ} e1 e2 :
-  (∀ σ1, if s.1 is NotStuck then reducible e1 σ1 else to_val e1 = None) →
+  (∀ σ1, if s is NotStuck then reducible e1 σ1 else to_val e1 = None) →
   (∀ σ1 κ e2' σ2 efs', prim_step e1 σ1 κ e2' σ2 efs' →
     κ = [] ∧ σ2 = σ1 ∧ e2' = e2 ∧ efs' = []) →
-  (|={E}[E']▷=> £ 1 -∗ (⚡={next_state (next_a e1 s.2)}=> WP e2 @ s; E {{ Φ }})) ⊢ WP e1 @ s; E {{ Φ }}.
+  (|={E}[E']▷=> £ 1 -∗ (⚡={next_state e1}=> WP e2 @ s; E {{ Φ }})) ⊢ WP e1 @ s; E {{ Φ }}.
 Proof.
   iIntros (? Hpuredet) "H". iApply (wp_lift_pure_step_no_fork s E E'); try done.
   { naive_solver. }
@@ -154,10 +154,10 @@ Proof.
   iIntros (κ e' efs' σ (_&?&->&?)%Hpuredet); auto.
 Qed.
 
-Fixpoint n_next_state (n : nat) (a : A) (P : iProp Σ) :=
+Fixpoint n_next_state (n : nat) (e1 : expr Λ) (P : iProp Σ) :=
   match n with
   | 0 => P
-  | S n => (⚡={next_state a}=> (n_next_state n a P))%I
+  | S n => (⚡={next_state e1}=> (n_next_state n e1 P))%I
   end.
 
 (* Lemma wp_pure_step_fupd `{!Inhabited (state Λ)} s E E' e1 e2 φ n Φ : *)
