src/nextgen_id.v
@@ -1,0 +1,22 @@
+From nextgen Require Import nextgen_basic.
+
+Import uPred.
+
+Section bnextgen_rules.
+  Context {M : ucmra}.
+
+  Notation "P ⊢ Q" := (@uPred_entails M P%I Q%I) : stdpp_scope.
+  Notation "⊢ Q" := (bi_entails (PROP:=uPredI M) True Q).
+  Notation "(⊢)" := (@uPred_entails M) (only parsing) : stdpp_scope.
+
+  Implicit Types (P Q : uPred M).
+
+  Local Arguments uPred_holds {_} !_ _ _ /.
+
+  Lemma nextgen_id P : (⚡={id}=> P) ⊣⊢ P.
+  Proof.
+    apply bnextgen_id.    
+    auto.
+  Qed.
+
+End bnextgen_rules.
